wip

src/Lean4Lean/Ext.lean
@@ -2,78 +2,128 @@ import Lean4Lean.RecM
 
 namespace Lean.TypeChecker.Inner
 
+open Lean.Meta
+
 def toKernelException (m : EIO Exception α) : EIO KernelException (Sum α Exception) := fun x =>
   match m x with
   | .ok s I => .ok (.inl s) I
   | .error e I => .ok (.inr e) I
 
-def runMetaM (m : MetaM T) : RecM T := do
-  let mut options := (← readThe Context).options
-  let m' := Lean.Meta.MetaM.run m {lctx := (← readThe Context).lctx, fuel := (← readThe Context).fuel - 1} |>.run {options := options, fileName := default, fileMap := default, maxHeartbeats := 0} {env := (← readThe Context).env'}
-  match ← toKernelException m' with
-  | .inl ((reqs, _), _) => pure reqs
-  | .inr (.internal _ _) => throw $ .other "untranslated Exception.Internal"
-  | .inr (.error _ d) => throw $ .other (← d.toString)
-
-def apply (mvarId : MVarId) (e : Expr) (eType? : Option Expr := none) : RecMO T (List MVarId) :=
-  mvarId.withContext do
-    mvarId.checkNotAssigned `apply
-    let targetType ← mvarId.getType
-    let eType      ← eType?.getDM (inferType e)
-    let (numArgs, hasMVarHead) ← getExpectedNumArgsAux eType
-    /-
-    The `apply` tactic adds `_`s to `e`, and some of these `_`s become new goals.
-    When `hasMVarHead` is `false` we try different numbers, until we find a type compatible with `targetType`.
-    We used to try only `numArgs-targetTypeNumArgs` when `hasMVarHead = false`, but this is not always correct.
-    For example, consider the following example
-    ```
-    example {α β} [LE_trans β] (x y z : α → β) (h₀ : x ≤ y) (h₁ : y ≤ z) : x ≤ z := by
-      apply le_trans
-      assumption
-      assumption
-    ```
-    In this example, `targetTypeNumArgs = 1` because `LE` for functions is defined as
-    ```
-    instance {α : Type u} {β : Type v} [LE β] : LE (α → β) where
-      le f g := ∀ i, f i ≤ g i
-    ```
-    -/
-    let rangeNumArgs ← if hasMVarHead then
-      pure [numArgs : numArgs+1]
+private def checkTypesAndAssign (mvar : Expr) (v : Expr) : RecMO T Bool := do
+  if !mvar.isMVar then
+    trace[Meta.isDefEq.assign.checkTypes] "metavariable expected"
+    return false
+  else
+    -- must check whether types are definitionally equal or not, before assigning and returning true
+    let mvarType ← inferType mvar
+    let vType ← inferType v
+    if (← Meta.isExprDefEqAux mvarType vType) then
+      mvar.mvarId!.assign v
+      pure true
     else
-      let targetTypeNumArgs ← getExpectedNumArgs targetType
-      pure [numArgs - targetTypeNumArgs : numArgs+1]
-    /-
-    Auxiliary function for trying to add `n` underscores where `n ∈ [i: rangeNumArgs.stop)`
-    See comment above
-    -/
-    let rec go (i : Nat) : MetaM (Array Expr × Array BinderInfo) := do
-      if i < rangeNumArgs.stop then
-        let s ← saveState
-        let (newMVars, binderInfos, eType) ← forallMetaTelescopeReducing eType i
-        if (← isDefEqApply cfg eType targetType) then
-          return (newMVars, binderInfos)
-        else
-          s.restore
-          go (i+1)
-      else
-        let (_, _, eType) ← forallMetaTelescopeReducing eType (some rangeNumArgs.start)
-        throwApplyError mvarId eType targetType
-      termination_by rangeNumArgs.stop - i
-    let (newMVars, binderInfos) ← go rangeNumArgs.start
-    postprocessAppMVars `apply mvarId newMVars binderInfos cfg.synthAssignedInstances cfg.allowSynthFailures
-    let e ← instantiateMVars e
-    mvarId.assign (mkAppN e newMVars)
-    let newMVars ← newMVars.filterM fun mvar => not <$> mvar.mvarId!.isAssigned
-    let otherMVarIds ← getMVarsNoDelayed e
-    let newMVarIds ← reorderGoals newMVars cfg.newGoals
-    let otherMVarIds := otherMVarIds.filter fun mvarId => !newMVarIds.contains mvarId
-    let result := newMVarIds ++ otherMVarIds.toList
-    result.forM (·.headBetaType)
-    return result
+      pure false
 
-open Lean.Meta in
-def extMatch (getT : MetaM (Expr × List Expr)) (localMarker : Name) (lems : List Name) (dbg := false) : RecMO T (Option (Expr × List Expr)) := do
+def isExprDefEqShallowImpl (t : Expr) (s : Expr) : RecMO T Bool :=
+  let rec processBinding (lctx : LocalContext) (fvars : Array Expr) (t s : Expr) : RecMO T Bool :=
+    let process (n : Name) (d₁ d₂ b₁ b₂ : Expr) : RecMO T Bool := do
+      let d₁     := d₁.instantiateRev fvars
+      let d₂     := d₂.instantiateRev fvars
+      if not (← isExprDefEqShallowImpl d₁ d₂) then
+        return false
+      let fvarId ← mkFreshFVarId
+      let lctx   := lctx.mkLocalDecl fvarId n d₁
+      let fvars  := fvars.push (mkFVar fvarId)
+      processBinding lctx fvars b₁ b₂
+    match t, s with
+    | .forallE n d₁ b₁ _,    .forallE _ d₂ b₂ _    => process n d₁ d₂ b₁ b₂
+    | .lam     n d₁ b₁ _,    .lam     _ d₂ b₂ _    => process n d₁ d₂ b₁ b₂
+    | .letE    n d₁ v₁ b₁ _, .letE    _ d₂ v₂ b₂ _ => isExprDefEqShallowImpl v₁ v₂ <&&> process n d₁ d₂ b₁ b₂
+    | _,                  _                  =>
+      withLCtx' lctx do
+        isExprDefEqShallowImpl (t.instantiateRev fvars) (s.instantiateRev fvars)
+  decreasing_by
+    sorry
+  match t, s with
+  | .lam .., .lam ..
+  | .forallE .., .forallE ..
+  | .letE .., .letE .. => do processBinding (← getLCtx) #[] t s
+  | .sort a1, .sort a2 => pure (a1.isEquiv a2)
+  | .mdata _ a1, _ => isExprDefEqShallowImpl a1 s
+  | _, .mdata _ a2 => isExprDefEqShallowImpl t a2
+  | .lit a1, .lit a2 => pure (a1 == a2)
+  | .proj n i s, .proj n' i' s' => pure (n == n') <&&> pure (i == i') <&&> isExprDefEqShallowImpl s s'
+  | .const n ls, .const n' ls' => pure (n == n' && (ls.zip ls').all (fun (l, l') => l.isEquiv l'))
+  | .fvar id, .fvar id' => pure $ id == id'
+  | .app f a, .app f' a' => isExprDefEqShallowImpl f f' <&&> isExprDefEqShallowImpl a a'
+  | .bvar .., _ => unreachable!
+  | _, .bvar .. => unreachable!
+  | .mvar .., .mvar .. => 
+    checkTypesAndAssign s t
+  | _, .mvar .. => 
+    checkTypesAndAssign s t
+  | .mvar .., _ =>
+    checkTypesAndAssign t s
+  | _, _ =>
+    pure false
+
+def apply (mvarId : MVarId) (e : Expr) (eType? : Option Expr := none) : RecMO T (List MVarId) := do
+  mvarId.checkNotAssigned `apply
+  let targetType ← mvarId.getType
+  let eType      ← eType?.getDM (inferType e)
+  let (numArgs, hasMVarHead) ← getExpectedNumArgsAux eType
+  /-
+  The `apply` tactic adds `_`s to `e`, and some of these `_`s become new goals.
+  When `hasMVarHead` is `false` we try different numbers, until we find a type compatible with `targetType`.
+  We used to try only `numArgs-targetTypeNumArgs` when `hasMVarHead = false`, but this is not always correct.
+  For example, consider the following example
+  ```
+  example {α β} [LE_trans β] (x y z : α → β) (h₀ : x ≤ y) (h₁ : y ≤ z) : x ≤ z := by
+    apply le_trans
+    assumption
+    assumption
+  ```
+  In this example, `targetTypeNumArgs = 1` because `LE` for functions is defined as
+  ```
+  instance {α : Type u} {β : Type v} [LE β] : LE (α → β) where
+    le f g := ∀ i, f i ≤ g i
+  ```
+  -/
+  let rangeNumArgs ← if hasMVarHead then
+    pure [numArgs : numArgs+1]
+  else
+    let targetTypeNumArgs ← getExpectedNumArgs targetType
+    pure [numArgs - targetTypeNumArgs : numArgs+1]
+  /-
+  Auxiliary function for trying to add `n` underscores where `n ∈ [i: rangeNumArgs.stop)`
+  See comment above
+  -/
+  let rec go (i : Nat) : MetaM (Array Expr × Array BinderInfo) := do
+    if i < rangeNumArgs.stop then
+      let s ← saveState
+      let (newMVars, binderInfos, eType) ← forallMetaTelescopeReducing eType i
+      if (← isDefEqApply cfg eType targetType) then
+        return (newMVars, binderInfos)
+      else
+        s.restore
+        go (i+1)
+    else
+      let (_, _, eType) ← forallMetaTelescopeReducing eType (some rangeNumArgs.start)
+      throwError "apply error: {mvarId} {eType} {targetType}"
+    termination_by rangeNumArgs.stop - i
+  let (newMVars, binderInfos) ← go rangeNumArgs.start
+  postprocessAppMVars `apply mvarId newMVars binderInfos cfg.synthAssignedInstances cfg.allowSynthFailures
+  let e ← instantiateMVars e
+  mvarId.assign (mkAppN e newMVars)
+  let newMVars ← newMVars.filterM fun mvar => not <$> mvar.mvarId!.isAssigned
+  let otherMVarIds ← getMVarsNoDelayed e
+  let newMVarIds ← reorderGoals newMVars cfg.newGoals
+  let otherMVarIds := otherMVarIds.filter fun mvarId => !newMVarIds.contains mvarId
+  let result := newMVarIds ++ otherMVarIds.toList
+  result.forM (·.headBetaType)
+  return result
+
+def extMatch (T : Expr) (ts : (List Expr)) (localMarker : Name) (lems : List Name) (dbg := false) : RecMO U (Option (Expr × List Expr)) := do
+
   if (← readThe Context).fuel == 0 then
     return none
   -- options := options.insert `trace.Meta.isDefEq (.ofBool true)
@@ -95,48 +145,46 @@ def extMatch (getT : MetaM (Expr × List Expr)) (localMarker : Name) (lems : Lis
 
     let mut candidates := (← lems.mapM (mkConstWithFreshMVarLevels ·)).zip (List.replicate lems.length none)
     candidates := candidates ++ localLems
-    liftM $ withLCtx' (← read).lctx do
-      let tryExtEq lem type? (T : Expr) (ts : List Expr) := do
-        let condString := do pure s!"{← ppExpr $ ← T.mvarId!.getType}"
-        -- let dbg := (← readThe Core.Context).options.get? `trace.Kernel.ext
-        trace[Kernel.ext] "Trying to show {← condString}"
-        try
-          trace[Kernel.ext] s!"Trying to apply (fuel {(← read).fuel}): {← ppExpr $ lem} : {← ppExpr $ (← Meta.inferType lem)} to {← condString}"
-          let gs ← T.mvarId!.apply lem (cfg := {shallow := true}) type?
+    let tryExtEq {U} lem type? (T : Expr) (ts : List Expr) : RecMO U (Option (Expr × List Expr)) := do
+      let condString := do pure s!"{← ppExpr $ ← T.mvarId!.getType}"
+      -- let dbg := (← readThe Core.Context).options.get? `trace.Kernel.ext
+      trace[Kernel.ext] "Trying to show {← condString}"
+      try
+        trace[Kernel.ext] s!"Trying to apply (fuel {(← read).fuel}): {← ppExpr $ lem} : {← ppExpr $ (← Meta.inferType lem)} to {← condString}"
+        let gs ← apply T.mvarId! lem type?
 
-          trace[Kernel.ext] s!"Applying OK:{← ppExpr $ (← Meta.inferType lem)} to  {← condString}" --"\n  {← gs.mapM (fun (id : MVarId) => do ppExpr $ ← id.getType)}\n  {← localLems.mapM (do ppExpr $ ← Meta.inferType ·.1)}"
-          if dbg then
-            dbg_trace s!"Applying OK:{← ppExpr $ (← Meta.inferType lem)} to  {← condString}" --"\n  {← gs.mapM (do ppExpr $ ← ·.getType)}\n  {← localLems.mapM (do ppExpr $ ← Meta.inferType ·.1)}"
-          for g in gs do
-            -- TODO unassign T if any g.refl fails?
-            try
-              trace[Kernel.ext] s!"Trying reflection: {← ppExpr $ ← g.getType}"
-              g.refl
-              trace[Kernel.ext] s!"Reflection OK: {← ppExpr $ ← g.getType}"
-            catch e =>
-              trace[Kernel.ext] s!"Reflection FAIL: {← ppExpr $ ← g.getType}"
-              throw e
-          trace[Kernel.ext] s!"Showing OK: {← ppExpr $ ← T.mvarId!.getType}"
-          let TInst ← instantiateMVars T
-          let tsInst ← ts.mapM fun t => instantiateMVars t
-          return some (TInst, tsInst)
-        catch e =>
-          trace[Kernel.ext] s!"Applying FAIL: {← ppExpr $ lem} : {← ppExpr $ (← Meta.inferType lem)} to {← condString}"
-          if dbg then
-            dbg_trace s!"Applying FAIL: {← ppExpr $ lem} : {← ppExpr $ (← Meta.inferType lem)} to {← condString}"
-          pure none
-      let (T, ts) ← getT
+        trace[Kernel.ext] s!"Applying OK:{← ppExpr $ (← Meta.inferType lem)} to  {← condString}" --"\n  {← gs.mapM (fun (id : MVarId) => do ppExpr $ ← id.getType)}\n  {← localLems.mapM (do ppExpr $ ← Meta.inferType ·.1)}"
+        if dbg then
+          dbg_trace s!"Applying OK:{← ppExpr $ (← Meta.inferType lem)} to  {← condString}" --"\n  {← gs.mapM (do ppExpr $ ← ·.getType)}\n  {← localLems.mapM (do ppExpr $ ← Meta.inferType ·.1)}"
+        for g in gs do
+          -- TODO unassign T if any g.refl fails?
+          try
+            trace[Kernel.ext] s!"Trying reflection: {← ppExpr $ ← g.getType}"
+            g.refl
+            trace[Kernel.ext] s!"Reflection OK: {← ppExpr $ ← g.getType}"
+          catch e =>
+            trace[Kernel.ext] s!"Reflection FAIL: {← ppExpr $ ← g.getType}"
+            throw e
+        trace[Kernel.ext] s!"Showing OK: {← ppExpr $ ← T.mvarId!.getType}"
+        let TInst ← instantiateMVars T
+        let tsInst ← ts.mapM (fun t => instantiateMVars t)
+        return some (TInst, tsInst)
+      catch e =>
+        trace[Kernel.ext] s!"Applying FAIL: {← ppExpr $ lem} : {← ppExpr $ (← Meta.inferType lem)} to {← condString}"
+        if dbg then
+          dbg_trace s!"Applying FAIL: {← ppExpr $ lem} : {← ppExpr $ (← Meta.inferType lem)} to {← condString}"
+        pure none
 
-      for (lem, type?) in candidates do
-        -- for eqMvar in [tEqsMvar, sEqtMvar] do
-        -- TODO is there a way to "undo" assignments from previous failed unification attempts,
-        -- rather than making new mvars every time?
-        if let .some prf ← tryExtEq lem type? T ts then
-          printTraces
-          return some prf
-      trace[Kernel.ext] "Showing FAIL: {← ppExpr $ ← T.mvarId!.getType}"
-      printTraces
-      return none
+    for (lem, type?) in candidates do
+      -- for eqMvar in [tEqsMvar, sEqtMvar] do
+      -- TODO is there a way to "undo" assignments from previous failed unification attempts,
+      -- rather than making new mvars every time?
+      if let .some prf ← tryExtEq lem type? T ts then
+        printTraces
+        return some prf
+    trace[Kernel.ext] "Showing FAIL: {← ppExpr $ ← T.mvarId!.getType}"
+    printTraces
+    return none
     )
 
   if let some (prf, ts) := ret? then
