src/Lean/Log.lean
@@ -12,7 +12,7 @@ namespace Lean
 /--
 The `MonadLog` interface for logging error messages.
 -/
-class MonadLog (m : Type → Type) extends MonadFileMap m where
+class MonadLog (m : Type → Type u) extends MonadFileMap m where
   /-- Return the current reference syntax being used to provide position information. -/
   getRef       : m Syntax
   /-- The name of the file being processed. -/
