src/Lean4Lean/RecM.lean
@@ -104,3 +104,9 @@ def whnfCore (e : Expr) (l : Option (Level × Expr) := none) (cheapRec := false)
 def whnf (e : Expr) (d : Option (Level × Expr) := none) : RecMO T Expr := fun f m => m.whnf e d fun e => f e m
 
 def inferType (e : Expr) (inferOnly := true) : RecMO T Expr := fun f m => m.inferType e inferOnly fun a => f a m
+
+instance : MonadTrace (RecMO T) :=
+  inferInstance
+
+instance : MonadMCtx (RecMO T) :=
+  inferInstance
